src/program_proof/single/try_decide_proof.v
@@ -12,8 +12,14 @@ Context `{paxosG Σ u64}.
 
 Context `{f:nat}.
 
+Definition is_Clerk (γ:single_names) (r:loc) (pid:nat) : iProp Σ.
+Admitted.
+
+Instance is_Clerk_pers r pid γ : Persistent (is_Clerk r pid γ).
+Admitted.
+
 Lemma wp_Clerk__Prepare ck pid γ reply_ptr dummy_rep (pn:u64) :
-  (* is_Clerk r pid γ -∗ *)
+  is_Clerk γ ck pid -∗
   {{{
        own_PrepareReply reply_ptr dummy_rep
   }}}
@@ -30,7 +36,7 @@ Proof.
 Admitted.
 
 Lemma wp_Clerk__Propose ck pid γ (pn:u64) (val:u64) :
-  (* is_Clerk r pid γ -∗ *)
+  is_Clerk γ ck pid -∗
   {{{
        pn_ptsto f γ (int.nat pn) val
   }}}
@@ -42,6 +48,35 @@ Lemma wp_Clerk__Propose ck pid γ (pn:u64) (val:u64) :
 Proof.
 Admitted.
 
+Context `{!ghost_mapG Σ nat unit}.
+
+Definition peers_prop γ (peers:list loc) : iProp Σ :=
+  ∃ (pids:list nat),
+  "#Hclerks" ∷ ([∗ list] ck;pid ∈ peers; pids, (is_Clerk γ ck pid)) ∗
+  "#HdistinctPeers" ∷ □(|==> ∃ γtok, [∗ list] pid ∈ pids, pid ↪[γtok] ())
+.
+
+Notation "'[∗' 'range]' n1 < x < n2 , P" := ([∗ set] x ∈ (fin_to_set u64),
+                                                   ⌜int.nat n1 ≤ int.nat x⌝ ∨
+                                           ⌜int.nat n2 ≤ int.nat x⌝ ∨
+                                           ((λ x, P) x))%I
+  (at level 200, n1 at level 10, n2 at level 10, x at level 1, right associativity,
+   format "[∗ range]  n1 < x < n2 ,  P") : bi_scope.
+
+Definition prepare_lock_inv γ γtok (pn:u64) (numPrepared_ptr highestVal_ptr highestPn_ptr:loc) : iProp Σ :=
+  ∃ (numPrepared highestPn:u64) (highestVal:u64) (S:gset nat),
+  "HnumPrepared" ∷ numPrepared_ptr ↦[uint64T] #numPrepared ∗
+  "HhighestPn" ∷ highestPn_ptr ↦[uint64T] #highestPn ∗
+  "HhighestVal" ∷ highestVal_ptr ↦[uint64T] #highestVal ∗
+  "%HpreparedSize" ∷ ⌜size S = int.nat numPrepared⌝ ∗
+  "Htoks" ∷ ([∗ set] pid ∈ S, pid ↪[γtok] ()) ∗
+  "#Hhighest_ptsto" ∷ pn_ptsto f γ (int.nat highestPn) highestVal ∗
+  "#Hrejected" ∷ ([∗ set] pid ∈ S,
+                  ([∗ range] highestPn < pn' < pn, rejected γ pid (int.nat pn')))
+                  (* ([∗ set] pn' ∈ (fin_to_set u64),
+      ⌜int.nat pn' ≤ int.nat highestPn⌝ ∨ ⌜int.nat pn ≤ int.nat pn'⌝ ∨
+      (rejected γ pid (int.nat pn)))) *)
+.
 
 Lemma wp_TryDecide s pid γ (v:u64) (outv_ptr:loc) :
   is_Replica s pid γ (f:=f) -∗
@@ -75,44 +110,101 @@ Proof.
 
   wp_apply (typed_mem.wp_AllocAt uint64T).
   { naive_solver. }
-  iIntros (numPrepared) "HnumPrepared".
+  iIntros (numPrepared_ptr) "HnumPrepared".
   wp_pures.
   wp_store.
 
   wp_apply (typed_mem.wp_AllocAt uint64T).
   { naive_solver. }
-  iIntros (highestPN) "HhighestPN".
+  iIntros (highestPN_ptr) "HhighestPN".
   wp_pures.
   wp_store.
 
   wp_apply (typed_mem.wp_AllocAt uint64T).
   { naive_solver. }
-  iIntros (highestVal) "HhighestVal".
+  iIntros (highestVal_ptr) "HhighestVal".
   wp_pures.
   wp_store.
 
   wp_apply (wp_new_free_lock).
   iIntros (l) "Hl".
   wp_pures.
-  Search (forSlice).
-  wp_loadField.
 
+  set (pn:=(word.add promisePN 1)).
+  iAssert (peers_prop γ peers) with "[]" as (pids) "HpeersProp".
+  { admit. } (* FIXME: this should be part of is_Replica *)
+  iNamed "HpeersProp".
+  iMod ("HdistinctPeers") as (γtok) "Hγtoks".
+  (* FIXME: this should not disappear *)
+
+  iMod (alloc_lock mutexN _ _ (prepare_lock_inv γ γtok pn numPrepared_ptr highestVal_ptr highestPN_ptr) with "Hl [HnumPrepared HhighestPN HhighestVal]").
+  {
+    iNext.
+    iExists _, _, _, ∅.
+    iFrame "∗#".
+    iSplitL ""; first done.
+    iSplitL "".
+    { iApply (big_sepS_empty). done. }
+    iSplitL ""; first admit. (* TODO: initial proposal *)
+    iApply (big_sepS_empty).
+    done.
+  }
+
+  wp_loadField.
   iMod (readonly_load with "HpeersSl") as (peersq) "HH".
-  wp_apply (wp_forSlice (λ _, True)%I with "[] [$HH]").
+  iDestruct (is_slice_small_sz with "HH") as %HpeersSz.
+
+  Search "wp_alloc".
+  Search struct.ptrT.
+  wp_apply (typed_slice.wp_forSlice (V:=loc) (λ i, [∗ list] k ↦ pid ∈ pids, ⌜k < int.nat i⌝ ∨ pid ↪[γtok] ()
+                        )%I with "[] [$HH Hγtoks]").
   {
     iIntros.
     clear Φ.
-    iIntros (Φ) "!# Hpre HΦ".
+    iIntros (Φ) "!# [Hpre [%HindexLe %Hlookup]] HΦ".
     wp_pures.
-    wp_apply (wp_fork).
+    iDestruct (big_sepL2_length with "Hclerks") as %HlengthEq.
+    assert (∃ ck, peers !! (int.nat i) = Some ck) as [ck Htemp].
+    {
+      apply list_lookup_lt.
+      rewrite -typed_slice.list_untype_length.
+      word.
+    }
+    iDestruct (big_sepL2_lookup_1_some with "Hclerks") as %Heq.
+    { done. }
+    destruct Heq as [pid' HpidLookup].
+    iDestruct (big_sepL_lookup_acc_impl (int.nat i) with "Hpre") as "[Hγtok Hγtoks]".
+    { naive_solver. }
+    iDestruct "Hγtok" as "[%Hbad|Hγtok]".
+    { exfalso. word. }
+    wp_apply (wp_fork with "[Hγtok]").
     {
       admit. (* FIXME: Will need per-thread token for updating state under mutex l *)
       (* Will make (I n) be ownership of all of the tokens except for the first n (exclusive) *)
     }
-    by iApply "HΦ".
+    iApply "HΦ".
+    iApply "Hγtoks".
+    {
+      iModIntro.
+      iIntros (????) "[%Hcase|$]".
+      iLeft; iPureIntro.
+      word.
+    }
+    iLeft.
+    iPureIntro.
+    clear -i HindexLe.
+    word. (* XXX: Because int.Z i < int.Z blah -> int.Z i < 2^64 - 1 *)
   }
+  {
+    iApply (big_sepL_impl with "Hγtoks").
+    iModIntro. iIntros.
+    iRight.
+    iFrame.
+  }
+
   iIntros "_".
-  wp_pures.
+
 Admitted.
+
 
 End try_decide_proof.
